Inserters/And.dfy
@@ -1,12 +1,10 @@
 module Inserters.And{
 
   import opened Circ
-  import opened Eval
-  import opened Utils
-  import opened Scuf
-  import opened Subcircuit
   import opened ConservedSubcircuit
   import opened MapFunction
+  import opened Inserters_Binary
+  import opened Modifiers.SwitchUF
 
   const AndUFConst := UpdateFunction(
     2, 1, 0,
@@ -20,171 +18,13 @@ module Inserters.And{
     AndUFConst
   }
 
-  function InsertAndImpl(c: Circuit): (r: (Circuit, Scuf))
-    requires c.Valid()
-    ensures r.0.Valid()
-    ensures r.1.SomewhatValid(r.0)
-    ensures r.1.MapValid()
-    ensures r.1.uf.Valid()
+  function AndInserter(): (z: ScufInserter)
+    ensures z.Valid()
   {
-    reveal Circuit.Valid();
-    var new_node := GetNewNode(c);
-    assert new_node !in c.NodeKind;
-    var new_c := Circuit(
-      NodeKind := c.NodeKind[new_node := CAnd],
-      PortSource := c.PortSource
-    );
-    var i_0 := NP(new_node, INPUT_0);
-    var i_1 := NP(new_node, INPUT_1);
-    var o_0 := NP(new_node, OUTPUT_0);
-    var inputs := [i_0, i_1];
-    var outputs := [o_0];
-    var state := [];
-    var mp := ScufMap(inputs, outputs, state);
-    assert mp.Valid() by {
-      reveal Seq.HasNoDuplicates();
-      reveal Seq.ToSet();
-    }
-    var uf := AndUF();
-    var s := Scuf({new_node}, mp, uf);
-    assert s.SomewhatValid(new_c) by {
-      reveal Scuf.SomewhatValid();
-      reveal Seq.ToSet();
-      reveal ScValid();
-      reveal ConnOutputs();
-      reveal ConnInputs();
-      reveal UnconnInputs();
-      reveal AllONPs();
-      reveal AllSeq();
-      assert ScValid(new_c, s.sc);
-      assert forall np: NP :: np.n in s.sc ==> np !in c.PortSource.Values;
-    }
-    assert s.MapValid() by {
-      reveal Seq.ToSet();
-      reveal NPsInSc();
-    }
-    (new_c, s)
-  }
-
-  lemma InsertAndF(c: Circuit, fi: FI)
-    requires c.Valid()
-    requires
-      var (new_c, s) := InsertAndImpl(c);
-      FIValid(fi, s.mp.inputs, s.mp.state)
-    ensures
-      var (new_c, s) := InsertAndImpl(c);
-      reveal Scuf.SomewhatValid();
-      reveal Seq.ToSet();
-      && s.f(fi) == FO(map[s.mp.outputs[0]:=fi.inputs[s.mp.inputs[0]] && fi.inputs[s.mp.inputs[1]]], map[])
-    {
-      reveal Scuf.SomewhatValid();
-      reveal Seq.ToSet();
-      reveal MapToSeq();
-      reveal SeqsToMap();
-    }
-      
-
-
-  lemma InsertAndCorrect(c: Circuit)
-    requires c.Valid()
-    ensures
-      var (new_c, e) := InsertAndImpl(c);
-      && e.Valid(new_c)
-  {
-    var (new_c, e) := InsertAndImpl(c);
-    var o := e.mp.outputs[0];
-    var i_0 := e.mp.inputs[0];
-    var i_1 := e.mp.inputs[1];
-    var path := [e.mp.outputs[0]];
-    assert PathValid(new_c, path) && PathValid(new_c, [o, i_0]) && PathValid(new_c, [o, i_1]) by {
-      reveal PathValid();
-    }
-    LengthOneNoDuplicates(path);
-    assert new_c.Valid();
-    reveal Seq.ToSet();
-    forall fi: FI | FIValid(fi, e.mp.inputs, e.mp.state)
-      ensures
-        var iv_0 := fi.inputs[i_0];
-        var iv_1 := fi.inputs[i_1];
-        && FICircuitValid(new_c, fi)
-        && (EvaluateONP(new_c, o, fi) == EvalOk(iv_0 && iv_1))
-    {
-      var iv_0 := fi.inputs[i_0];
-      var iv_1 := fi.inputs[i_1];
-      assert Seq.HasNoDuplicates(path);
-      assert FICircuitValid(new_c, fi) by {
-        reveal UpdateFunction.Valid();
-        reveal FICircuitValid();
-      }
-      assert EvaluateONP(new_c, o, fi) == EvaluateONPBinary(new_c, [o], fi);
-      reveal Seq.HasNoDuplicates();
-      assert EvaluateINPInner(new_c, [o, i_0], fi) == EvalOk(iv_0);
-      assert EvaluateINPInner(new_c, [o, i_1], fi) == EvalOk(iv_1);
-      assert EvaluateONPBinary(new_c, [o], fi) == EvalOk(iv_0 && iv_1);
-      assert EvaluateONPInner(new_c, [o], fi) == EvalOk(iv_0 && iv_1);
-      assert EvaluateONP(new_c, o, fi) == EvalOk(iv_0 && iv_1);
-      assert Evaluate(new_c, o, fi) == EvalOk(iv_0 && iv_1);
-      assert Evaluate(new_c, o, fi) == EvalOk(e.f(fi).outputs[o]) by {
-        InsertAndF(c, fi);
-      }
-    }
-    assert ScValid(new_c, e.sc) by {
-      reveal Scuf.SomewhatValid();
-    }
-    assert e.EvaluatesCorrectly(new_c) by {
-      reveal Scuf.EvaluatesCorrectly();
-      reveal MapMatchesSeqs();
-    }
-    assert e.Valid(new_c);
-  }
-
-  lemma InsertAndConserves(c: Circuit)
-    requires c.Valid()
-    ensures CircuitConserved(c, InsertAndImpl(c).0)
-    ensures CircuitUnconnected(c, InsertAndImpl(c).0)
-    ensures
-      var (new_c, e) := InsertAndImpl(c);
-      IsIsland(new_c, e.sc)
-  {
-    reveal CircuitConserved();
-    reveal CircuitUnconnected();
-    var (new_c, e) := InsertAndImpl(c);
-    reveal Circuit.Valid();
-    assert (forall np :: np in c.PortSource.Keys ==> np.n !in e.sc);
-    assert (forall np :: np in c.PortSource.Values ==> np.n !in e.sc);
-    assert (forall np :: np in new_c.PortSource && np.n in e.sc ==> new_c.PortSource[np].n in e.sc);
-    assert (forall np :: np in new_c.PortSource && np.n !in e.sc ==> new_c.PortSource[np].n !in e.sc);
-    reveal IsIsland();
-  }
-
-  function InsertAnd(c: Circuit): (r: (Circuit, Scuf))
-    requires c.Valid()
-    ensures
-      var (new_c, e) := r;
-      && r == InsertAndImpl(c)
-      && r.0.Valid()
-      && e.Valid(new_c)
-      && CircuitConserved(c, r.0)
-      && CircuitUnconnected(c, r.0)
-      && IsIsland(new_c, e.sc)
-  {
-    InsertAndCorrect(c);
-    InsertAndConserves(c);
-    InsertAndImpl(c)
-  }
-
-  const AndInserterConst := ScufInserter(AndUF(), InsertAnd)
-
-  function AndInserter(): (r: ScufInserter)
-    ensures r.Valid()
-  {
-    reveal UpdateFunction.Valid();
-    reveal ScufInserter.Valid();
-    var z := AndInserterConst;
-    assert z.Valid() by {
-      reveal SimpleInsertion();
-    }
-    z 
+    var z_binary := BinaryInserter(CAnd);
+    reveal UpdateFunctionsEquiv();
+    var z := SwitchUFModifier(z_binary, AndUF());
+    z_binary
   }
 
 }
